Use singletons rather than sets

extract/Main.hs
@@ -26,12 +26,12 @@ w82c = toEnum . fromIntegral
 w82s :: [Word8] -> String
 w82s = map w82c
 
--- printPS :: Rep -> CRep -> BScrep -> IO String
--- printPS h h' bs =
---     let (bs', mres) = unconsBS h h' bs in
---     case mres of
---         Nothing -> return []
---         Just c  -> (w82c c:) <$> printPS h h' bs'
+printPS :: Rep -> CRep -> BScrep -> IO String
+printPS h h' bs =
+    let (bs', mres) = unconsBS h h' bs in
+    case mres of
+        Nothing -> return []
+        Just c  -> (w82c c:) <$> printPS h h' bs'
 
 printPS0 :: PS0 -> IO String
 printPS0 bs =
@@ -53,22 +53,25 @@ main = do
     let (_h4, val) = peekHeap h3 (of_nat 105)
     print val
 
-    -- putStrLn "ByteString list..."
+    putStrLn "ByteString list..."
 
-    -- let b0 = emptyBS any' h0
-    -- putStrLn . ("b0 = " ++) =<< printPS any' h0 b0
-    -- let b1 = consBS any' h0 b0 (c2w8 'a')
-    -- putStrLn . ("b1 = " ++) =<< printPS any' h0 b1
-    -- let b2 = consBS any' h0 b1 (c2w8 'b')
-    -- putStrLn . ("b2 = " ++) =<< printPS any' h0 b2
-    -- let b3 = consBS any' h0 b2 (c2w8 'c')
-    -- putStrLn . ("b3 = " ++) =<< printPS any' h0 b3
-    -- let (b4, mres1) = unconsBS any' h0 b3
-    -- putStrLn . ("b4 = " ++) =<< printPS any' h0 b4
-    -- print mres1
-    -- let (b5, mres2) = unconsBS any' h0 b4
-    -- putStrLn . ("b5 = " ++) =<< printPS any' h0 b5
-    -- print mres2
+    let b0 = emptyBS any' h0
+    putStrLn . ("b0 = " ++) =<< printPS any' h0 b0
+    let b1 = consBS any' h0 b0 (c2w8 'a')
+    putStrLn . ("b1 = " ++) =<< printPS any' h0 b1
+    let b2 = consBS any' h0 b1 (c2w8 'b')
+    putStrLn . ("b2 = " ++) =<< printPS any' h0 b2
+    let b3 = consBS any' h0 b2 (c2w8 'c')
+    putStrLn . ("b3 = " ++) =<< printPS any' h0 b3
+    let (b4, mres1) = unconsBS any' h0 b3
+    putStrLn . ("b4 = " ++) =<< printPS any' h0 b4
+    print mres1
+    let (b5, mres2) = unconsBS any' h0 b4
+    putStrLn . ("b5 = " ++) =<< printPS any' h0 b5
+    print mres2
+
+    let b6 = appendBS any' h0 b2 b3
+    putStrLn . ("bs6 = " ++) =<< printPS any' h0 b6
 
     putStrLn "ByteString heap..."
 
