src/ByteStringCanon.v
@@ -43,14 +43,12 @@ Lemma refine_ByteString_Heap_AbsR :
   forall heap_resvs heap_bytes buffer buflen offset length B (k : _ -> Comp B),
     refineEquiv
       (r_n' <- { r_n0 : cHeapRep * PS
-               | forall oh : HeapState,
-                   ret {| resvs := heap_resvs
-                        ; bytes := heap_bytes |} ↝ oh ->
-                   Heap_AbsR oh (fst r_n0) /\
-                   {| psBuffer := buffer
-                    ; psBufLen := buflen
-                    ; psOffset := offset
-                    ; psLength := length |} = snd r_n0 };
+               | Heap_AbsR {| resvs := heap_resvs
+                            ; bytes := heap_bytes |} (fst r_n0) /\
+                 {| psBuffer := buffer
+                  ; psBufLen := buflen
+                  ; psOffset := offset
+                  ; psLength := length |} = snd r_n0 };
        k r_n')
       (resvs' <- {resvs' : M.t Size | M.Equal heap_resvs resvs'};
        bytes' <- {bytes' : M.t Word | M.Equal heap_bytes bytes'};
@@ -75,11 +73,9 @@ Proof.
       apply refine_computes_to.
       assumption.
     rewrite HeqP.
-    intros; destruct_computations.
     firstorder.
   intros; intros ??.
   destruct_computations.
-  specialize (H _ (ReturnComputes _)).
   destruct H, x; simpl in *.
   subst.
   remember (makePS _ _ _ _) as P; intros.
@@ -104,14 +100,12 @@ Lemma refine_ByteString_Heap_AbsR' :
   forall heap_resvs heap_bytes buffer buflen offset length,
     refineEquiv
       { r_n0 : cHeapRep * PS
-      | forall oh : HeapState,
-          ret {| resvs := heap_resvs
-               ; bytes := heap_bytes |} ↝ oh ->
-          Heap_AbsR oh (fst r_n0) /\
-          {| psBuffer := buffer
-           ; psBufLen := buflen
-           ; psOffset := offset
-           ; psLength := length |} = snd r_n0 }
+      | Heap_AbsR {| resvs := heap_resvs
+                   ; bytes := heap_bytes |} (fst r_n0) /\
+        {| psBuffer := buffer
+         ; psBufLen := buflen
+         ; psOffset := offset
+         ; psLength := length |} = snd r_n0 }
       (resvs' <- {resvs' : M.t Size | M.Equal heap_resvs resvs'};
        bytes' <- {bytes' : M.t Word | M.Equal heap_bytes bytes'};
        brk'   <- {brk'   : N
@@ -133,11 +127,9 @@ Proof.
       apply refine_computes_to.
       constructor.
     rewrite HeqP.
-    intros; destruct_computations.
     firstorder.
   intros; intros ??.
   destruct_computations.
-  specialize (H _ (ReturnComputes _)).
   destruct H, v; simpl in *.
   subst.
   remember (makePS _ _ _ _) as P; intros.
@@ -161,10 +153,10 @@ Qed.
 
 Ltac apply_ByteString_Heap_AbsR :=
   match goal with
-    | [ H : Heap_AbsR ?O (fst ?N) /\ snd ?X = snd ?Y |- _ ] =>
+    | [ H : Heap_AbsR (fst ?O) (fst ?N) /\ snd ?X = snd ?Y |- _ ] =>
       destruct H as
           [ [ resvs_match0 [ bytes_match0 for_all_matches0 ] ] match0 ],
-          O as [ resvs_o bytes_o ];
+          O as [ [ resvs_o bytes_o ] ps_o ];
       simpl in *;
       rewrite ?match0
   end.
@@ -182,12 +174,10 @@ Tactic Notation "refine" "using" "ByteString_Heap_AbsR" :=
         | [ |- refine (x <- ret _; _) _ ] =>
           simplify with monad laws; simpl
         | [ |- refine (x <- { X : cHeapRep * PS
-                            | forall oh : HeapState, _ ↝ oh
-                                -> Heap_AbsR oh (fst X) /\ _ = snd X }; _) _ ] =>
+                            | Heap_AbsR _ (fst X) /\ _ = snd X }; _) _ ] =>
           rewrite refine_ByteString_Heap_AbsR
         | [ |- refine { X : cHeapRep * PS
-                      | forall oh : HeapState, _ ↝ oh
-                          -> Heap_AbsR oh (fst X) /\ _ = snd X } _ ] =>
+                      | Heap_AbsR _ (fst X) /\ _ = snd X } _ ] =>
           rewrite refine_ByteString_Heap_AbsR'
         | [ |- refine (If ?B Then ?T Else ?E) _ ] =>
           apply refine_If_Then_Else
@@ -207,14 +197,14 @@ Tactic Notation "refine" "using" "ByteString_Heap_AbsR" :=
     end
   end.
 
+Variable only_one_heap : forall h1 h2 : Rep HeapSpec, h1 = h2.
+
 Theorem ByteStringCanonical : FullySharpened (projT1 (ByteStringHeap heap)).
 Proof.
   start sharpening ADT.
 
   hone representation using
-       (fun (or : Comp (Rep HeapSpec) * PS) (nr : cHeapRep * PS) =>
-          forall oh, fst or ↝ oh ->
-            Heap_AbsR oh (fst nr) /\ snd or = snd nr).
+       (fun or nr => Heap_AbsR (fst or) (fst nr) /\ snd or = snd nr).
 
   (* refine method ByteString.emptyS. *)
   {
@@ -224,107 +214,61 @@ Proof.
                              ; psOffset := 0
                              ; psLength := 0 |}).
       finish honing.
-    simpl; intuition.
-    destruct_computations.
-    assumption.
+    firstorder.
   }
 
   (* refine method ByteString.consS. *)
   {
-    simplify with monad laws.
-    etransitivity.
-      apply refine_under_bind; intros.
-      specialize (H0 _ H1); clear H1.
-      apply_ByteString_Heap_AbsR.
-      fracture H.
-      etransitivity.
-      {
-        refine using ByteString_Heap_AbsR;
-        unfold find_free_block;
-        refine pick val (fst (fst r_n)); eauto;
-        try simplify with monad laws;
-        try finish honing;
-        refine using ByteString_Heap_AbsR;
-        (rewrite resvs_match0;
-         eapply for_all_impl; eauto;
-         relational; simpl; intros;
-         clear -H0; nomega).
-      }
-      etransitivity.
-      {
-        apply refine_If_Then_Else.
-          reflexivity.
-        apply refine_If_Then_Else.
-          reflexivity.
-        apply refine_If_Then_Else.
-        - refine using ByteString_Heap_AbsR.
-          refine pick val (plusPtr (A:=Word) (fst (fst r_n))
-                                   (psLength (snd r_n) + alloc_quantum)); eauto.
-            simplify with monad laws.
-            finish honing.
+    apply_ByteString_Heap_AbsR.
+    fracture H; unfold find_free_block;
+    refine using ByteString_Heap_AbsR;
+    refine pick val (fst (fst r_n)); eauto;
+    try simplify with monad laws;
+    try finish honing;
+    refine using ByteString_Heap_AbsR.
 
-          rewrite <- remove_add.
-          apply for_all_remove; relational.
-            rewrite H0; reflexivity.
-          apply for_all_add_true; relational; try nomega.
-              rewrite H0; reflexivity.
-            simplify_maps.
-          split; [|clear; nomega].
-          apply for_all_remove; relational; try nomega.
-            rewrite H0; reflexivity.
-          eapply for_all_impl; auto;
-          relational; eauto;
-          rewrite ?H0; clear; nomega.
+    - refine pick val (plusPtr (A:=Word) (fst (fst r_n))
+                               (psLength (snd r_n) + alloc_quantum)); eauto.
+        simplify with monad laws.
+        finish honing.
 
-        - refine using ByteString_Heap_AbsR.
-          refine pick val (plusPtr (A:=Word) (fst (fst r_n)) alloc_quantum); eauto.
-            simplify with monad laws.
-            finish honing.
+      rewrite <- remove_add.
+      apply for_all_remove; relational.
+        rewrite H; reflexivity.
+      apply for_all_add_true; relational; try nomega.
+        simplify_maps.
+      split; [|nomega].
+      apply for_all_remove; relational; try nomega.
+      eapply for_all_impl; auto;
+      relational; eauto; nomega.
 
-          rewrite <- remove_add.
-          apply for_all_add_true; relational; try nomega.
-              rewrite H0; reflexivity.
-            simplify_maps.
-          split; [|clear; nomega].
-          apply for_all_remove; relational; try nomega.
-            rewrite H0; reflexivity.
-          eapply for_all_impl; auto;
-          relational; eauto;
-          rewrite ?H0; clear; nomega.
-      }
+    - rewrite resvs_match0.
+      eapply for_all_impl; eauto;
+      relational; nomega.
 
-      rewrite !refine_If_Then_Else_ret.
-      finish honing.
+    - refine pick val (plusPtr (A:=Word) (fst (fst r_n)) alloc_quantum); eauto.
+        simplify with monad laws.
+        finish honing.
 
-    simpl.
-    Fail finish honing.
-    admit.
+      rewrite <- remove_add.
+      apply for_all_add_true; relational; try nomega.
+        simplify_maps.
+      split; [|nomega].
+      apply for_all_remove; relational; try nomega.
+      eapply for_all_impl; auto;
+      relational; eauto; nomega.
+
+    - rewrite resvs_match0.
+      eapply for_all_impl; eauto;
+      relational; nomega.
   }
 
   (* refine method ByteString.unconsS. *)
   {
-    admit.
-(*
-    simplify with monad laws.
-    etransitivity.
-      apply refine_under_bind; intros.
-      specialize (H0 _ H1); clear H1.
-      apply_ByteString_Heap_AbsR.
-      fracture H.
-      etransitivity.
-      etransitivity.
-      {
-        refine using ByteString_Heap_AbsR;
-        unfold find_free_block.
-        refine pick val (fst (fst r_n)); eauto;
-        try simplify with monad laws;
-        try finish honing;
-        refine using ByteString_Heap_AbsR;
-        (rewrite resvs_match0;
-         eapply for_all_impl; eauto;
-         relational; simpl; intros;
-         clear -H0; nomega).
-      }
+    unfold buffer_uncons;
+    apply_ByteString_Heap_AbsR;
+    fracture H;
+    refine using ByteString_Heap_AbsR.
 
     - refine pick val (Ifopt M.find (plusPtr (A:=Word) (psBuffer (snd r_n))
                                              (psOffset (snd r_n)))
@@ -352,15 +296,18 @@ Proof.
         finish honing.
       split; trivial.
       constructor; auto.
-*)
   }
 
   (* refine method ByteString.appendS. *)
   {
     unfold buffer_append, alloc, Bind2, find_free_block; simpl.
 
-    admit.
-(*
+    simplify with monad laws.
+    refine_under.
+      apply refine_pick_val.
+      rewrite only_one_heap with (h1:=fst r_o) (h2:=fst r_o0).
+      split; reflexivity.
+
     rewrite !refine_IfDep_Then_Else_Bind,
             !refineEquiv_strip_IfDep_Then_Else.
     refine pick val (plusPtr (A:=Word) (fst (fst r_n)) 1).
@@ -372,10 +319,10 @@ Proof.
             simplify with monad laws; simpl.
             destruct H0, H1.
             rewrite e, e0; clear e e0.
-            destruct h, H1, h0, H4.
+            destruct h, H1, h0, H5.
             refine pick val
               ((plusPtr (A:=Word) (fst (fst r_n))
-                        (psLength (snd r_n) + psLength (snd r_n0) + 1),
+                        (1 + psLength (snd r_n) + psLength (snd r_n0)),
                 {| resvs := M.add (plusPtr (A:=Word) (fst (fst r_n)) 1)
                                   (psLength (snd r_n) + psLength (snd r_n0))
                                   (resvs (snd (fst r_n)))
@@ -383,16 +330,15 @@ Proof.
                      copy_bytes (A:=Word)
                        (plusPtr (A:=Word) (psBuffer (snd r_n0))
                                 (psOffset (snd r_n0)))
-                       (plusPtr (A:=Word) (fst (fst r_n))
-                                (psLength (snd r_n) + 1))
+                       (plusPtr (A:=Word)
+                                (plusPtr (A:=Word) (fst (fst r_n)) 1)
+                                (psLength (snd r_n)))
                        (psLength (snd r_n0))
-                       (bytes (snd (fst r_n0)))
                        (copy_bytes (A:=Word)
                                    (plusPtr (A:=Word) (psBuffer (snd r_n))
                                             (psOffset (snd r_n)))
                                    (plusPtr (A:=Word) (fst (fst r_n)) 1)
                                    (psLength (snd r_n))
-                                   (bytes (snd (fst r_n)))
                                    (bytes (snd (fst r_n)))) |}),
                {| psBuffer := plusPtr (A:=Word) (fst (fst r_n)) 1
                 ; psBufLen := psLength (snd r_n) + psLength (snd r_n0)
@@ -406,9 +352,12 @@ Proof.
               rewrite H0.
               reflexivity.
             split.
-              rewrite H1, H4.
+              rewrite H1.
+              replace (plusPtr (A:=Word) (fst (fst r_n)) 1 + psLength (snd r_n))
+                 with (plusPtr (A:=Word) (fst (fst r_n)) (psLength (snd r_n) + 1))
+                   by nomega.
               reflexivity.
-            clear -H2.
+            clear -H3.
             apply for_all_add_true; relational; try nomega.
               destruct 1.
               apply_for_all; relational.
@@ -427,19 +376,18 @@ Proof.
           finish honing.
         assumption.
       intuition.
-      rewrite !H3, !H4.
+      rewrite !H4, !H5.
       rewrite !refine_If_Then_Else_ret.
       finish honing.
     intuition.
-    rewrite H3, H4.
-    destruct H2.
+    rewrite H4, H5.
+    destruct H3.
     rewrite H1.
     intuition.
     clear -H6.
     remember (fun _ _ => _) as P.
     remember (fun _ _ => negb _) as P'.
     apply for_all_impl with (P:=P) (P':=P'); relational; nomega.
-*)
   }
 
   (** Apply some common functional optimizations, such as common subexpression
@@ -468,12 +416,9 @@ Proof.
     simplify with monad laws.
     refine pick eq.
     simplify with monad laws.
-    admit.
-(*
     rewrite !If_Then_Else_fst, !If_Then_Else_snd; simpl.
     rewrite If_Then_Else_pair.
     subst; finish honing.
-*)
   }
 
   (* refine method ByteString.appendS. *)
@@ -483,8 +428,10 @@ Proof.
   }
 
   finish_SharpeningADT_WithoutDelegation.
-(* Defined. *)
-Admitted.
+
+  Unshelve.
+  constructor.
+Defined.
 
 End Refined.
 
